converted to Isar theory format;

src/HOLCF/IOA/Storage/Action.thy
@@ -1,10 +1,19 @@
 (*  Title:      HOLCF/IOA/ABP/Action.thy
     ID:         $Id$
     Author:     Olaf Müller
-
-The set of all actions of the system.
 *)
 
-Action =  Main +
-datatype action = New  | Loc nat | Free nat        
+header {* The set of all actions of the system *}
+
+theory Action
+imports Main
+begin
+
+datatype action = New  | Loc nat | Free nat
+
+lemma [cong]: "!!x. x = y ==> action_case a b c x = action_case a b c y"
+  by simp
+
+ML {* use_legacy_bindings (the_context ()) *}
+
 end
