src/HOLCF/IOA/ABP/Abschannel_finite.thy
@@ -1,78 +1,64 @@
 (*  Title:      HOLCF/IOA/ABP/Abschannels.thy
     ID:         $Id$
     Author:     Olaf Müller
-
-The transmission channel -- finite version.
 *)
 
-Abschannel_finite = Abschannel+ IOA + Action + Lemmas + List +
- 
+header {* The transmission channel -- finite version *}
+
+theory Abschannel_finite
+imports Abschannel IOA Action Lemmas
+begin
+
 consts
- 
+
 ch_fin_asig  :: "'a abs_action signature"
 
-ch_fin_trans :: ('a abs_action, 'a list)transition set
+ch_fin_trans :: "('a abs_action, 'a list)transition set"
 
-ch_fin_ioa   :: ('a abs_action, 'a list)ioa
+ch_fin_ioa   :: "('a abs_action, 'a list)ioa"
 
-srch_fin_asig, 
+srch_fin_asig  :: "'m action signature"
 rsch_fin_asig  :: "'m action signature"
 
-srch_fin_trans :: ('m action, 'm packet list)transition set
-rsch_fin_trans :: ('m action, bool list)transition set
+srch_fin_trans :: "('m action, 'm packet list)transition set"
+rsch_fin_trans :: "('m action, bool list)transition set"
 
-srch_fin_ioa   :: ('m action, 'm packet list)ioa
-rsch_fin_ioa   :: ('m action, bool list)ioa   
+srch_fin_ioa   :: "('m action, 'm packet list)ioa"
+rsch_fin_ioa   :: "('m action, bool list)ioa"
 
-reverse        :: 'a list => 'a list
+reverse        :: "'a list => 'a list"
 
 primrec
-  reverse_Nil  "reverse([]) = []"
-  reverse_Cons "reverse(x#xs) =  reverse(xs)@[x]"
+  reverse_Nil:  "reverse([]) = []"
+  reverse_Cons: "reverse(x#xs) =  reverse(xs)@[x]"
 
 defs
 
-srch_fin_asig_def "srch_fin_asig == asig_of(srch_fin_ioa)"
-rsch_fin_asig_def "rsch_fin_asig == asig_of(rsch_fin_ioa)"
+srch_fin_asig_def: "srch_fin_asig == asig_of(srch_fin_ioa)"
+rsch_fin_asig_def: "rsch_fin_asig == asig_of(rsch_fin_ioa)"
 
-srch_fin_trans_def "srch_fin_trans == trans_of(srch_fin_ioa)"  
-rsch_fin_trans_def "rsch_fin_trans == trans_of(rsch_fin_ioa)"
+srch_fin_trans_def: "srch_fin_trans == trans_of(srch_fin_ioa)"
+rsch_fin_trans_def: "rsch_fin_trans == trans_of(rsch_fin_ioa)"
 
-srch_fin_ioa_def "srch_fin_ioa == rename ch_fin_ioa  srch_actions"
-rsch_fin_ioa_def "rsch_fin_ioa == rename ch_fin_ioa  rsch_actions"
+srch_fin_ioa_def: "srch_fin_ioa == rename ch_fin_ioa  srch_actions"
+rsch_fin_ioa_def: "rsch_fin_ioa == rename ch_fin_ioa  rsch_actions"
 
 
-ch_fin_asig_def "ch_fin_asig == ch_asig"
+ch_fin_asig_def: "ch_fin_asig == ch_asig"
 
-ch_fin_trans_def "ch_fin_trans ==                                       
- {tr. let s = fst(tr);                                         
-          t = snd(snd(tr))                                     
-      in                                                       
-      case fst(snd(tr))                                        
-        of S(b) => ((t = s) |                                    
-                   (if (b=hd(reverse(s)) & s~=[]) then  t=s else  t=s@[b])) |    
-           R(b) => s ~= [] &                                   
-                    b = hd(s) &                                 
+ch_fin_trans_def: "ch_fin_trans ==
+ {tr. let s = fst(tr);
+          t = snd(snd(tr))
+      in
+      case fst(snd(tr))
+        of S(b) => ((t = s) |
+                   (if (b=hd(reverse(s)) & s~=[]) then  t=s else  t=s@[b])) |
+           R(b) => s ~= [] &
+                    b = hd(s) &
                     ((t = s) | (t = tl(s)))    }"
-  
-ch_fin_ioa_def "ch_fin_ioa == (ch_fin_asig, {[]}, ch_fin_trans,{},{})"
 
-end  
+ch_fin_ioa_def: "ch_fin_ioa == (ch_fin_asig, {[]}, ch_fin_trans,{},{})"
 
+ML {* use_legacy_bindings (the_context ()) *}
 
-
-
-
-
-
-
-
-
-
-
-
-
-
-
-
-
+end
