src/HOLCF/IOA/ABP/Env.thy
@@ -1,46 +1,43 @@
 (*  Title:      HOLCF/IOA/ABP/Impl.thy
     ID:         $Id$
     Author:     Olaf Müller
-
-The environment.
 *)
 
-Env = IOA + Action +
+header {* The environment *}
+
+theory Env
+imports IOA Action
+begin
 
 types
+  'm env_state = bool   -- {* give next bit to system *}
 
-'m env_state = "bool"
-(*              give next bit to system  *)
-
-consts
-
+constdefs
 env_asig   :: "'m action signature"
-env_trans  :: ('m action, 'm env_state)transition set
-env_ioa    :: ('m action, 'm env_state)ioa
-next       :: 'm env_state => bool
-
-defs
-
-env_asig_def
-  "env_asig == ({Next},                 
-               UN m. {S_msg(m)},       
+"env_asig == ({Next},
+               UN m. {S_msg(m)},
                {})"
 
-env_trans_def "env_trans ==                                           
- {tr. let s = fst(tr);                                               
-          t = snd(snd(tr))                                           
-      in case fst(snd(tr))                                           
-      of                                                             
-      Next       => t=True |                                         
-      S_msg(m)   => s=True & t=False |                               
-      R_msg(m)   => False |                                          
-      S_pkt(pkt) => False |                                          
-      R_pkt(pkt) => False |                                          
-      S_ack(b)   => False |                                          
+env_trans  :: "('m action, 'm env_state)transition set"
+"env_trans ==
+ {tr. let s = fst(tr);
+          t = snd(snd(tr))
+      in case fst(snd(tr))
+      of
+      Next       => t=True |
+      S_msg(m)   => s=True & t=False |
+      R_msg(m)   => False |
+      S_pkt(pkt) => False |
+      R_pkt(pkt) => False |
+      S_ack(b)   => False |
       R_ack(b)   => False}"
 
-env_ioa_def "env_ioa == 
- (env_asig, {True}, env_trans,{},{})"
+env_ioa    :: "('m action, 'm env_state)ioa"
+"env_ioa == (env_asig, {True}, env_trans,{},{})"
+
+consts
+  "next"     :: "'m env_state => bool"
+
+ML {* use_legacy_bindings (the_context ()) *}
 
 end
-
