src/HOLCF/IOA/ABP/Impl.thy
@@ -1,34 +1,35 @@
 (*  Title:      HOLCF/IOA/ABP/Impl.thy
     ID:         $Id$
     Author:     Olaf Müller
-
-The implementation.
 *)
 
-Impl = Sender + Receiver +  Abschannel +
+header {* The implementation *}
 
-types 
+theory Impl
+imports Sender Receiver Abschannel
+begin
 
-'m impl_state 
-= "'m sender_state * 'm receiver_state * 'm packet list * bool list"
-(*  sender_state   *  receiver_state   *    srch_state  * rsch_state *)
-
+types
+  'm impl_state = "'m sender_state * 'm receiver_state * 'm packet list * bool list"
+  (*  sender_state   *  receiver_state   *    srch_state  * rsch_state *)
 
 constdefs
 
- impl_ioa    :: ('m action, 'm impl_state)ioa
+ impl_ioa    :: "('m action, 'm impl_state)ioa"
  "impl_ioa == (sender_ioa || receiver_ioa || srch_ioa || rsch_ioa)"
 
- sen         :: 'm impl_state => 'm sender_state
+ sen         :: "'m impl_state => 'm sender_state"
  "sen == fst"
 
- rec         :: 'm impl_state => 'm receiver_state
+ rec         :: "'m impl_state => 'm receiver_state"
  "rec == fst o snd"
 
- srch        :: 'm impl_state => 'm packet list
+ srch        :: "'m impl_state => 'm packet list"
  "srch == fst o snd o snd"
 
- rsch        :: 'm impl_state => bool list
+ rsch        :: "'m impl_state => bool list"
  "rsch == snd o snd o snd"
+
+ML {* use_legacy_bindings (the_context ()) *}
 
 end
