src/HOLCF/IOA/ABP/Impl_finite.thy
@@ -1,35 +1,37 @@
 (*  Title:      HOLCF/IOA/ABP/Impl.thy
     ID:         $Id$
     Author:     Olaf Müller
-
-The implementation.
 *)
 
-Impl_finite = Sender + Receiver +  Abschannel_finite +
-  
-types 
+header {* The implementation *}
 
-'m impl_fin_state 
-= "'m sender_state * 'm receiver_state * 'm packet list * bool list"
+theory Impl_finite
+imports Sender Receiver Abschannel_finite
+begin
+
+types
+  'm impl_fin_state
+    = "'m sender_state * 'm receiver_state * 'm packet list * bool list"
 (*  sender_state   *  receiver_state   *    srch_state  * rsch_state *)
 
 constdefs
 
- impl_fin_ioa    :: ('m action, 'm impl_fin_state)ioa
+ impl_fin_ioa    :: "('m action, 'm impl_fin_state)ioa"
  "impl_fin_ioa == (sender_ioa || receiver_ioa || srch_fin_ioa ||
                    rsch_fin_ioa)"
 
- sen_fin         :: 'm impl_fin_state => 'm sender_state
+ sen_fin         :: "'m impl_fin_state => 'm sender_state"
  "sen_fin == fst"
 
- rec_fin         :: 'm impl_fin_state => 'm receiver_state
+ rec_fin         :: "'m impl_fin_state => 'm receiver_state"
  "rec_fin == fst o snd"
 
- srch_fin        :: 'm impl_fin_state => 'm packet list
+ srch_fin        :: "'m impl_fin_state => 'm packet list"
  "srch_fin == fst o snd o snd"
 
- rsch_fin        :: 'm impl_fin_state => bool list
+ rsch_fin        :: "'m impl_fin_state => bool list"
  "rsch_fin == snd o snd o snd"
 
-end
+ML {* use_legacy_bindings (the_context ()) *}
 
+end
