src/HOLCF/IOA/ABP/Lemmas.thy
@@ -1,8 +1,10 @@
 (*  Title:      HOLCF/IOA/ABP/Lemmas.thy
     ID:         $Id$
     Author:     Olaf Müller
-
-Arithmetic lemmas.
 *)
 
-Lemmas = Main
+theory Lemmas
+imports Main
+begin
+
+end
