src/HOLCF/IOA/ABP/Packet.thy
@@ -1,22 +1,24 @@
 (*  Title:      HOLCF/IOA/ABP/Packet.thy
     ID:         $Id$
     Author:     Olaf Müller
-
-Packets.
 *)
 
-Packet = NatArith +
+header {* Packets *}
+
+theory Packet
+imports Main
+begin
 
 types
-
-   'msg packet = "bool * 'msg"
+  'msg packet = "bool * 'msg"
 
 constdefs
-
-  hdr  :: 'msg packet => bool
+  hdr  :: "'msg packet => bool"
   "hdr == fst"
 
-  msg :: 'msg packet => 'msg
+  msg :: "'msg packet => 'msg"
   "msg == snd"
+
+ML {* use_legacy_bindings (the_context ()) *}
 
 end
