src/HOLCF/IOA/ABP/Receiver.thy
@@ -1,58 +1,56 @@
 (*  Title:      HOLCF/IOA/ABP/Receiver.thy
     ID:         $Id$
     Author:     Olaf Müller
-
-The implementation: receiver.
 *)
 
-Receiver = List + IOA + Action + Lemmas +
+header {* The implementation: receiver *}
 
-types 
+theory Receiver
+imports IOA Action Lemmas
+begin
 
-'m receiver_state
-= "'m list * bool"
-(* messages  mode *)
+types
+  'm receiver_state = "'m list * bool"  -- {* messages, mode *}
 
-consts
+constdefs
+  rq            :: "'m receiver_state => 'm list"
+  "rq == fst"
 
-  receiver_asig :: "'m action signature"
-  receiver_trans:: ('m action, 'm receiver_state)transition set
-  receiver_ioa  :: ('m action, 'm receiver_state)ioa
-  rq            :: 'm receiver_state => 'm list
-  rbit          :: 'm receiver_state => bool
+  rbit          :: "'m receiver_state => bool"
+  "rbit == snd"
 
-defs
-
-rq_def       "rq == fst"
-rbit_def     "rbit == snd"
-
-receiver_asig_def "receiver_asig ==            
- (UN pkt. {R_pkt(pkt)},                       
-  (UN m. {R_msg(m)}) Un (UN b. {S_ack(b)}),   
+receiver_asig :: "'m action signature"
+"receiver_asig ==
+  (UN pkt. {R_pkt(pkt)},
+  (UN m. {R_msg(m)}) Un (UN b. {S_ack(b)}),
   {})"
 
-receiver_trans_def "receiver_trans ==                                    
- {tr. let s = fst(tr);                                                  
-          t = snd(snd(tr))                                              
-      in                                                                
-      case fst(snd(tr))                                                 
-      of   
-      Next    =>  False |     
-      S_msg(m) => False |                                               
-      R_msg(m) => (rq(s) ~= [])  &                                     
-                   m = hd(rq(s))  &                             
-                   rq(t) = tl(rq(s))   &                              
-                  rbit(t)=rbit(s)  |                                 
-      S_pkt(pkt) => False |                                          
-      R_pkt(pkt) => if (hdr(pkt) ~= rbit(s))&rq(s)=[] then            
-                         rq(t) = (rq(s)@[msg(pkt)]) &rbit(t) = (~rbit(s)) else  
-                         rq(t) =rq(s) & rbit(t)=rbit(s)  |   
-      S_ack(b) => b = rbit(s)                        &               
-                      rq(t) = rq(s)                    &             
-                      rbit(t)=rbit(s) |                              
+receiver_trans :: "('m action, 'm receiver_state)transition set"
+"receiver_trans ==
+ {tr. let s = fst(tr);
+          t = snd(snd(tr))
+      in
+      case fst(snd(tr))
+      of
+      Next    =>  False |
+      S_msg(m) => False |
+      R_msg(m) => (rq(s) ~= [])  &
+                   m = hd(rq(s))  &
+                   rq(t) = tl(rq(s))   &
+                  rbit(t)=rbit(s)  |
+      S_pkt(pkt) => False |
+      R_pkt(pkt) => if (hdr(pkt) ~= rbit(s))&rq(s)=[] then
+                         rq(t) = (rq(s)@[msg(pkt)]) &rbit(t) = (~rbit(s)) else
+                         rq(t) =rq(s) & rbit(t)=rbit(s)  |
+      S_ack(b) => b = rbit(s)                        &
+                      rq(t) = rq(s)                    &
+                      rbit(t)=rbit(s) |
       R_ack(b) => False}"
 
-receiver_ioa_def "receiver_ioa == 
+receiver_ioa :: "('m action, 'm receiver_state)ioa"
+"receiver_ioa ==
  (receiver_asig, {([],False)}, receiver_trans,{},{})"
+
+ML {* use_legacy_bindings (the_context ()) *}
 
 end
