src/HOLCF/IOA/ABP/Sender.thy
@@ -1,56 +1,54 @@
 (*  Title:      HOLCF/IOA/ABP/Sender.thy
     ID:         $Id$
     Author:     Olaf Müller
-
-The implementation: sender.
 *)
 
-Sender = IOA + Action + List + Lemmas +
+header {* The implementation: sender *}
+
+theory Sender
+imports IOA Action Lemmas
+begin
 
 types
+  'm sender_state = "'m list  *  bool"  -- {* messages, Alternating Bit *}
 
-'m sender_state = "'m list  *  bool"
-(*                messages     Alternating Bit   *)
+constdefs
+sq            :: "'m sender_state => 'm list"
+"sq == fst"
 
-consts
+sbit          :: "'m sender_state => bool"
+"sbit == snd"
 
 sender_asig   :: "'m action signature"
-sender_trans  :: ('m action, 'm sender_state)transition set
-sender_ioa    :: ('m action, 'm sender_state)ioa
-sq            :: 'm sender_state => 'm list
-sbit          :: 'm sender_state => bool
-
-defs
-
-sq_def       "sq == fst"
-sbit_def     "sbit == snd"
-
-sender_asig_def
-  "sender_asig == ((UN m. {S_msg(m)}) Un (UN b. {R_ack(b)}),       
-                  UN pkt. {S_pkt(pkt)},                   
+"sender_asig == ((UN m. {S_msg(m)}) Un (UN b. {R_ack(b)}),
+                  UN pkt. {S_pkt(pkt)},
                   {})"
 
-sender_trans_def "sender_trans ==                                     
- {tr. let s = fst(tr);                                               
-          t = snd(snd(tr))                                           
-      in case fst(snd(tr))                                           
-      of   
-      Next     => if sq(s)=[] then t=s else False |                
-      S_msg(m) => sq(t)=sq(s)@[m]   &                                
-                  sbit(t)=sbit(s)  |                                 
-      R_msg(m) => False |                                            
-      S_pkt(pkt) => sq(s) ~= []  &                                   
-                     hdr(pkt) = sbit(s)      &                        
-                    msg(pkt) = hd(sq(s))    &                   
-                    sq(t) = sq(s)           &                        
-                    sbit(t) = sbit(s) |                              
-      R_pkt(pkt) => False |                                          
-      S_ack(b)   => False |                                          
-      R_ack(b)   => if b = sbit(s) then                              
-                     sq(t)=tl(sq(s)) & sbit(t)=(~sbit(s)) else   
+sender_trans  :: "('m action, 'm sender_state)transition set"
+"sender_trans ==
+ {tr. let s = fst(tr);
+          t = snd(snd(tr))
+      in case fst(snd(tr))
+      of
+      Next     => if sq(s)=[] then t=s else False |
+      S_msg(m) => sq(t)=sq(s)@[m]   &
+                  sbit(t)=sbit(s)  |
+      R_msg(m) => False |
+      S_pkt(pkt) => sq(s) ~= []  &
+                     hdr(pkt) = sbit(s)      &
+                    msg(pkt) = hd(sq(s))    &
+                    sq(t) = sq(s)           &
+                    sbit(t) = sbit(s) |
+      R_pkt(pkt) => False |
+      S_ack(b)   => False |
+      R_ack(b)   => if b = sbit(s) then
+                     sq(t)=tl(sq(s)) & sbit(t)=(~sbit(s)) else
                      sq(t)=sq(s) & sbit(t)=sbit(s)}"
 
-sender_ioa_def "sender_ioa == 
+sender_ioa    :: "('m action, 'm sender_state)ioa"
+"sender_ioa ==
  (sender_asig, {([],True)}, sender_trans,{},{})"
+
+ML {* use_legacy_bindings (the_context ()) *}
 
 end
