src/HOLCF/IOA/Modelcheck/MuIOA.thy
@@ -1,16 +1,20 @@
 
-MuIOA = IOA + MuckeSyn +
+(* $Id$ *)
+
+theory MuIOA
+imports IOA MuckeSyn
+begin
 
 consts
-  Internal_of_A :: 'a => bool
-  Internal_of_C :: 'a => bool
-  Start_of_A :: 'a => bool
-  Start_of_C :: 'a => bool
-  Trans_of_A :: 'a => 'b => bool
-  Trans_of_C :: 'a => 'b => bool
-  IntStep_of_A :: 'a => bool
-  IntStepStar_of_A :: 'a => bool
-  Move_of_A :: 'a => 'b => bool
-  isSimCA :: 'a => bool
+  Internal_of_A :: "'a => bool"
+  Internal_of_C :: "'a => bool"
+  Start_of_A :: "'a => bool"
+  Start_of_C :: "'a => bool"
+  Trans_of_A :: "'a => 'b => bool"
+  Trans_of_C :: "'a => 'b => bool"
+  IntStep_of_A :: "'a => bool"
+  IntStepStar_of_A :: "'a => bool"
+  Move_of_A :: "'a => 'b => bool"
+  isSimCA :: "'a => bool"
 
 end
