src/HOLCF/IOA/NTP/Action.thy
@@ -1,13 +1,19 @@
 (*  Title:      HOL/IOA/NTP/Action.thy
     ID:         $Id$
     Author:     Tobias Nipkow & Konrad Slind
-
-The set of all actions of the system.
 *)
 
-Action = Packet + Datatype +
-datatype 'm action = S_msg ('m) | R_msg ('m)
-                   | S_pkt ('m packet) | R_pkt ('m packet)
-                   | S_ack (bool) | R_ack (bool)
-                   | C_m_s | C_m_r | C_r_s | C_r_r ('m)
+header {* The set of all actions of the system *}
+
+theory Action
+imports Packet
+begin
+
+datatype 'm action = S_msg 'm | R_msg 'm
+                   | S_pkt "'m packet" | R_pkt "'m packet"
+                   | S_ack bool | R_ack bool
+                   | C_m_s | C_m_r | C_r_s | C_r_r 'm
+
+ML {* use_legacy_bindings (the_context ()) *}
+
 end
