src/HOLCF/IOA/NTP/Correctness.thy
@@ -1,16 +1,19 @@
 (*  Title:      HOL/IOA/NTP/Correctness.thy
     ID:         $Id$
     Author:     Tobias Nipkow & Konrad Slind
-
-The main correctness proof: Impl implements Spec.
 *)
 
-Correctness = Impl + Spec +
+header {* The main correctness proof: Impl implements Spec *}
+
+theory Correctness
+imports Impl Spec
+begin
 
 constdefs
-
-  hom :: 'm impl_state => 'm list
-  "hom(s) == rq(rec(s)) @ (if rbit(rec s) = sbit(sen s) then sq(sen s) 
+  hom :: "'m impl_state => 'm list"
+  "hom(s) == rq(rec(s)) @ (if rbit(rec s) = sbit(sen s) then sq(sen s)
                            else tl(sq(sen s)))"
+
+ML {* use_legacy_bindings (the_context ()) *}
 
 end
