src/HOLCF/IOA/NTP/Lemmas.thy
@@ -1,8 +1,11 @@
 (*  Title:      HOL/IOA/NTP/Lemmas.thy
     ID:         $Id$
     Author:     Tobias Nipkow & Konrad Slind
-
-Arithmetic lemmas.
 *)
 
-Lemmas = NatArith
+theory Lemmas
+imports Main
+begin
+
+end
+
