src/HOLCF/IOA/NTP/Multiset.thy
@@ -1,47 +1,47 @@
 (*  Title:      HOL/IOA/NTP/Multiset.thy
     ID:         $Id$
     Author:     Tobias Nipkow & Konrad Slind
-
-Axiomatic multisets.
-Should be done as a subtype and moved to a global place.
 *)
 
-Multiset = Lemmas +
+header {* Axiomatic multisets *}
 
-types
+theory Multiset
+imports Lemmas
+begin
 
+typedecl
   'a multiset
-
-arities
-
-  multiset :: (type) type
 
 consts
 
-  "{|}"  :: 'a multiset                        ("{|}")
-  addm   :: ['a multiset, 'a] => 'a multiset
-  delm   :: ['a multiset, 'a] => 'a multiset
-  countm :: ['a multiset, 'a => bool] => nat
-  count  :: ['a multiset, 'a] => nat
+  "{|}"  :: "'a multiset"                        ("{|}")
+  addm   :: "['a multiset, 'a] => 'a multiset"
+  delm   :: "['a multiset, 'a] => 'a multiset"
+  countm :: "['a multiset, 'a => bool] => nat"
+  count  :: "['a multiset, 'a] => nat"
 
-rules
+axioms
 
-delm_empty_def
-  "delm {|} x = {|}" 
+delm_empty_def:
+  "delm {|} x = {|}"
 
-delm_nonempty_def
+delm_nonempty_def:
   "delm (addm M x) y == (if x=y then M else addm (delm M y) x)"
 
-countm_empty_def
+countm_empty_def:
    "countm {|} P == 0"
 
-countm_nonempty_def
+countm_nonempty_def:
    "countm (addm M x) P == countm M P + (if P x then Suc 0 else 0)"
 
-count_def
+count_def:
    "count M x == countm M (%y. y = x)"
 
-induction
+"induction":
    "[| P({|}); !!M x. P(M) ==> P(addm M x) |] ==> P(M)"
+
+ML {* use_text Context.ml_output true
+  ("structure Multiset = struct " ^ legacy_bindings (the_context ()) ^ " end") *}
+ML {* open Multiset *}
 
 end
