src/HOLCF/IOA/NTP/Packet.thy
@@ -1,22 +1,23 @@
 (*  Title:      HOL/IOA/NTP/Packet.thy
     ID:         $Id$
     Author:     Tobias Nipkow & Konrad Slind
-
-Packets.
 *)
 
-Packet = Multiset +  
+theory Packet
+imports Multiset
+begin
 
 types
-
-   'msg packet = "bool * 'msg"
+  'msg packet = "bool * 'msg"
 
 constdefs
 
-  hdr  :: 'msg packet => bool
+  hdr  :: "'msg packet => bool"
   "hdr == fst"
 
-  msg :: 'msg packet => 'msg
+  msg :: "'msg packet => 'msg"
   "msg == snd"
+
+ML {* use_legacy_bindings (the_context ()) *}
 
 end
