src/HOLCF/IOA/Storage/Impl.thy
@@ -1,12 +1,13 @@
 (*  Title:      HOL/IOA/example/Spec.thy
     ID:         $Id$
     Author:     Olaf Müller
-
-The implementation of a memory.
 *)
 
-Impl = IOA + Action +
+header {* The implementation of a memory *}
 
+theory Impl
+imports IOA Action
+begin
 
 consts
 
@@ -16,20 +17,28 @@ impl_ioa   :: "(action, nat * bool)ioa"
 
 defs
 
-sig_def "impl_sig == (UN l.{Free l} Un {New}, 
-                     UN l.{Loc l}, 
+sig_def: "impl_sig == (UN l.{Free l} Un {New},
+                     UN l.{Loc l},
                      {})"
 
-trans_def "impl_trans ==                           
- {tr. let s = fst(tr); k = fst s; b = snd s;                            
-          t = snd(snd(tr)); k' = fst t; b' = snd t                      
-      in                                          
-      case fst(snd(tr))                           
-      of   
-      New       => k' = k & b'  |                    
-      Loc l     => b & l= k & k'= (Suc k) & ~b' |                    
+trans_def: "impl_trans ==
+ {tr. let s = fst(tr); k = fst s; b = snd s;
+          t = snd(snd(tr)); k' = fst t; b' = snd t
+      in
+      case fst(snd(tr))
+      of
+      New       => k' = k & b'  |
+      Loc l     => b & l= k & k'= (Suc k) & ~b' |
       Free l    => k'=k & b'=b}"
 
-ioa_def "impl_ioa == (impl_sig, {(0,False)}, impl_trans,{},{})"
+ioa_def: "impl_ioa == (impl_sig, {(0,False)}, impl_trans,{},{})"
+
+lemma in_impl_asig:
+  "New : actions(impl_sig) &
+    Loc l : actions(impl_sig) &
+    Free l : actions(impl_sig) "
+  by (simp add: Impl.sig_def actions_def asig_projections)
+
+ML {* use_legacy_bindings (the_context ()) *}
 
 end
