src/HOLCF/IOA/Storage/Spec.thy
@@ -1,12 +1,13 @@
 (*  Title:      HOL/IOA/example/Spec.thy
     ID:         $Id$
     Author:     Olaf Müller
-
-The specification of a memory.
 *)
 
-Spec = IOA + Action +
+header {* The specification of a memory *}
 
+theory Spec
+imports IOA Action
+begin
 
 consts
 
@@ -16,20 +17,22 @@ spec_ioa   :: "(action, nat set * bool)ioa"
 
 defs
 
-sig_def "spec_sig == (UN l.{Free l} Un {New}, 
-                     UN l.{Loc l}, 
+sig_def: "spec_sig == (UN l.{Free l} Un {New},
+                     UN l.{Loc l},
                      {})"
 
-trans_def "spec_trans ==                           
- {tr. let s = fst(tr); used = fst s; c = snd s;                            
-          t = snd(snd(tr)); used' = fst t; c' = snd t                      
-      in                                          
-      case fst(snd(tr))                           
-      of   
-      New       => used' = used & c'  |                    
-      Loc l     => c & l~:used  & used'= used Un {l} & ~c'   |                    
+trans_def: "spec_trans ==
+ {tr. let s = fst(tr); used = fst s; c = snd s;
+          t = snd(snd(tr)); used' = fst t; c' = snd t
+      in
+      case fst(snd(tr))
+      of
+      New       => used' = used & c'  |
+      Loc l     => c & l~:used  & used'= used Un {l} & ~c'   |
       Free l    => used'=used - {l} & c'=c}"
 
-ioa_def "spec_ioa == (spec_sig, {({},False)}, spec_trans,{},{})"
+ioa_def: "spec_ioa == (spec_sig, {({},False)}, spec_trans,{},{})"
+
+ML {* use_legacy_bindings (the_context ()) *}
 
 end
