src/HOLCF/IOA/ex/TrivEx.thy
@@ -1,60 +1,64 @@
 (*  Title:      HOLCF/IOA/TrivEx.thy
     ID:         $Id$
     Author:     Olaf Müller
-
-Trivial Abstraction Example.
 *)
 
-TrivEx = Abstraction + 
+header {* Trivial Abstraction Example *}
+
+theory TrivEx
+imports Abstraction
+begin
 
 datatype action = INC
 
 consts
 
 C_asig   ::  "action signature"
-C_trans  :: (action, nat)transition set
-C_ioa    :: (action, nat)ioa
+C_trans  :: "(action, nat)transition set"
+C_ioa    :: "(action, nat)ioa"
 
 A_asig   :: "action signature"
-A_trans  :: (action, bool)transition set
-A_ioa    :: (action, bool)ioa
+A_trans  :: "(action, bool)transition set"
+A_ioa    :: "(action, bool)ioa"
 
 h_abs    :: "nat => bool"
 
 defs
 
-C_asig_def
+C_asig_def:
   "C_asig == ({},{INC},{})"
 
-C_trans_def "C_trans ==                                           
- {tr. let s = fst(tr);                                               
-          t = snd(snd(tr))                                           
-      in case fst(snd(tr))                                           
-      of                                                             
+C_trans_def: "C_trans ==
+ {tr. let s = fst(tr);
+          t = snd(snd(tr))
+      in case fst(snd(tr))
+      of
       INC       => t = Suc(s)}"
 
-C_ioa_def "C_ioa == 
+C_ioa_def: "C_ioa ==
  (C_asig, {0}, C_trans,{},{})"
 
-A_asig_def
+A_asig_def:
   "A_asig == ({},{INC},{})"
 
-A_trans_def "A_trans ==                                           
- {tr. let s = fst(tr);                                               
-          t = snd(snd(tr))                                           
-      in case fst(snd(tr))                                           
-      of                                                             
+A_trans_def: "A_trans ==
+ {tr. let s = fst(tr);
+          t = snd(snd(tr))
+      in case fst(snd(tr))
+      of
       INC       => t = True}"
 
-A_ioa_def "A_ioa == 
+A_ioa_def: "A_ioa ==
  (A_asig, {False}, A_trans,{},{})"
 
-h_abs_def
+h_abs_def:
   "h_abs n == n~=0"
 
-rules
+axioms
 
-MC_result
+MC_result:
   "validIOA A_ioa (<>[] <%(b,a,c). b>)"
+
+ML {* use_legacy_bindings (the_context ()) *}
 
 end
